Below is an example of a system of linear equations.
$$
\begin{align}
x_{1}-2x_{2} &= -1 \\
-x_{1}+3x_{2} &= 3
\end{align}
$$
The solution set to the above system is $\{ (3,2) \}$. 

A system of linear equations
1. has exactly one solution,
2. has infinitely many solutions, or,
3. has no solution.

If the system has at least one solution, it is said to be consistent. Otherwise, it is inconsistent.

## Matrix Notation

Given the system,

$$
\begin{align}
x_{1} - 2x_{2} + x_{3} = 0 \\
2x_{2} - 8x_{3} = 8 \\
5x_{1} - 5x_{3} = 10 
\end{align}
$$

we can construct a **coefficient matrix** as follows -

$$
\begin{bmatrix}
1 & -2 & 1 \\
0 & 2 & 8 \\
5 & 0 & -5
\end{bmatrix}
$$

The **augmented matrix**, with the right hand sides of the equations, is given below.

$$
\begin{bmatrix}
1 & -2 & 1 & 0 \\
0 & 2 & 8 & 8 \\
5 & 0 & -5 & 10
\end{bmatrix}
$$

## Making new Taylor Series 

Theorem A $C^\infty$ function hsa a unique power series expansion centered at $x=a$.
Corollary - No matter how you get it, the power series will be the same.

We can use substitution. For example,

$$
e^x= \sum_{n=0}^{\infty}  \frac{1}{n!}x^n
$$

for all $x \in \mathbb{R}$.

$$
\frac{1}{1-x} = \sum_{n=0}^{\infty} x^n
$$

only for $|x|<1$. So,

$$
e^{-t^2} = \sum_{n=o}^{\infty} \frac{1}{n!}(-t^{2})^n=\sum_{n=0}^{\infty} \frac{(-1)^n}{n!}t^{2n}
$$

true for all $t$. So, this is the taylor series for $e^{-t^{2}}$.
Eg.

$$
\frac{d^{27}}{dt^{27}} e^{-t^2} = 0
$$

Since coefficient for $t^{27}$ is 0. (We see that from the power series derived before). This means that if you get any power series, it has to be equal to the taylor series of the function.

## Basic Taylor Power Series

$$
e^x= \sum_{n=0}^{\infty} \frac{1}{n!}x^n
$$
$$
\sin(x) = \sum_{n=0}^{\infty} \frac{(-1)^n}{(2n+1)!}x^{2n+1}
$$
$$
\cos(x) = \sum_{n=0}^{\infty} \frac{(-1)^n}{(2n)!}x^{2n}
$$
$$
\frac{1}{1-x} = \sum_{n=0}^{\infty} x^n, 
$$

## Sub:

$$
\frac{1}{1+x^2} = \frac{1}{1-(-x^2)} = \sum_{n=0}^{\infty} (-x^{2})^n = \sum_{n=0}^{\infty} (-1)^nx^{2n} 
$$

Warning:

$$
f(x) = e^{-1/x^{2}}
$$

as $x\to 0$, $-\frac{1}{x^2} \to -\infty$, $e^{-1/x^2} \to 0$

We can show that 

$$
f^{(n)}(0) = 0
$$

Therefore, the taylor expansion,

$$
P(x) = \sum_{n=0}^{\infty}  \frac{0}{n!}x^n
$$

Take Taylor Polynomials $P_{n}(x)$, the error does not go to 0.

Apparently Complex Analysis explains it very well. 

## Formal Derivatives and Integrals

$$
P(x) = \sum_{n=0}^{\infty} a_{n}(x-a)^n
$$
$$
FI(P(x)) = \sum_{n=0}^{\infty} \frac{a_{n}}{n+1}(x-a)^{n+1}
$$

Here, the degree 0 coefficient is zero.

$$
FD(P(x)) = \sum_{n=0}^{\infty} a_{n}(n)(x-a)^{n-1}
$$

Degree 0 is the $n=1$ term.

Theorem: On the open interval of convergence of $P(x)$,

$$
FI(P(x)) = \int_{a}^{x} P(t) \, dt 
$$
$$
FD(P(x)) = P'(x)
$$

Example:

$$
\frac{d}{dx} \arctan(x) = \frac{1}{1+x^2} = \sum_{n=0}^{\infty} (-1)^nx^{2n}
$$
$$
\int_{0}^{x} \frac{1}{1+t^2} \, dt = \int_{0}^{x} \sum_{n=0}^{\infty} (-1)^nt^{2n} \, dt = \sum_{n=0}^{\infty} \frac{(-1)^n}{2n+1}x^{2n+1} = \arctan(x) + C = \arctan(x)  
$$

## "Easy Fact"

$P'(x)$ and $\int_{a}^{x} P(t) \, dt$ have the same interval of convergence. (Do the ratio test)

$$
\arctan(1) = \frac{\pi}{4}
$$
$$
\frac{\pi}{4} = \sum_{n=0}^{\infty} (-1)^n \frac{1^{2n+1}}{2n+1} = 1 - \frac{1}{3} +\frac{1}{5} - \frac{1}{7} +\dots
$$